qcp/ast/annotated_C/subst.c
@@ -1,18 +1,53 @@
 #include "ast.h"
 
+/*@ Import Coq From SimpleC.EE Require Import ast_lib */
+/*@ Import Coq From SimpleC.EE Require Import malloc */
+/*@ Import Coq From SimpleC.EE Require Import sll_tmpl */
+
+/*@ Extern Coq (var_name :: *)*/
+/*@ Extern Coq (const_type :: *)*/
+/*@ Extern Coq (quant_type :: *)*/
+/*@ Extern Coq (term_type :: *)*/
+/*@ Extern Coq (store_term : Z -> term -> Assertion)
+               (store_string : Z -> list Z -> Assertion)
+               (ctID : const_type -> Z)
+               (qtID : quant_type -> Z)
+               (ttID : term_type -> Z)
+               (termtypeID : term -> Z)
+               (TermVar: list Z -> term)
+               (TermConst: const_type -> Z -> term)
+               (TermApply: term -> term -> term)
+               (TermQuant: quant_type -> list Z -> term -> term)
+*/
+
 term *subst_var(char *den, char *src, term *t)
-/*@ With term src_str den_str
-      Require store_term(t, term) *
+/*@ With trm src_str den_str
+      Require den != 0 && src != 0 && t != 0 &&
+              store_term(t, trm) *
               store_string(src, src_str) *
               store_string(den, den_str)
       Ensure __return == t && t == t@pre && den == den@pre && src == src@pre &&
-             store_term(t, term_subst_v(den, src, term)) *
+             store_term(t, term_subst_v(den_str, src_str, trm)) *
              store_string(den, den_str) *
              store_string(src, src_str)
 */
 {
+  /*@ store_term(t, trm) 
+      which implies
+        data_at(&(t -> type), termtypeID(trm)) *
+        store_term'(t, trm)
+  */
   switch (t->type) {
     case Var: {
+      /*@ data_at(&(t -> type), termtypeID(trm)) *
+          store_term'(t, trm)
+          which implies
+          exists y var,
+            trm == TermVar(var) &&
+            data_at(&(t -> type), termtypeID(trm)) *
+            data_at(&(t -> content.Var), y) *
+            store_string(y, var)
+      */
       if (!strcmp(t->content.Var, src)) {
         free_str(t->content.Var);
         t->content.Var = strdup(den);
@@ -23,11 +58,32 @@ term *subst_var(char *den, char *src, term *t)
       break;
     }
     case Apply: {
+      /*@ data_at(&(t -> type), termtypeID(trm)) *
+          store_term'(t, trm)
+          which implies
+          exists y z lt rt,
+            trm == TermApply(lt, rt) &&
+            data_at(&(t -> type), termtypeID(trm)) *
+            data_at(&(t -> content.Apply.left), y) *
+            data_at(&(t -> content.Apply.right), z) *
+            store_term(y, lt) * store_term(z, rt)
+      */
       t->content.Apply.left = subst_var(den, src, t->content.Apply.left);
       t->content.Apply.right = subst_var(den, src, t->content.Apply.right);
       break;
     }
     case Quant: {
+      /*@ data_at(&(t -> type), termtypeID(trm)) *
+          store_term'(t, trm)
+          which implies
+          exists y z qt qvar qterm,
+            trm == TermQuant(qt, qvar, qterm) &&
+            data_at(&(t -> type), termtypeID(trm)) *
+            data_at(&(t -> content.Quant.type), qtID(qt)) *
+            data_at(&(t -> content.Quant.var), y) *
+            data_at(&(t -> content.Quant.body), z) *
+            store_string(y, qvar) * store_term(z, qterm)
+      */
       if (strcmp(t->content.Quant.var, src)) {
         t->content.Quant.body = subst_var(den, src, t->content.Quant.body);
       }
@@ -41,18 +97,42 @@ term *subst_var(char *den, char *src, term *t)
 }
 
 term *subst_term(term *den, char *src, term *t)
-/*@ With term src_str den_term
-      Require store_term(t, term) *
+/*@ With trm src_str den_term
+      Require den != 0 && src != 0 && t != 0 &&
+              store_term(t, trm) *
               store_string(src, src_str) *
               store_term(den, den_term)
       Ensure __return == t && t == t@pre && den == den@pre && src == src@pre &&
-             store_term(t, term_subst_t(den, src, term)) *
+             store_term(t, term_subst_t(den_term, src_str, trm)) *
              store_term(den, den_term) *
              store_string(src, src_str)
-*/{
+*/
+{
+  /*@ store_term(t, trm) 
+      which implies
+        data_at(&(t -> type), termtypeID(trm)) *
+        store_term'(t, trm)
+  */
   switch (t->type) {
     case Var: {
+      /*@ data_at(&(t -> type), termtypeID(trm)) *
+          store_term'(t, trm)
+          which implies
+          exists y var,
+            trm == TermVar(var) &&
+            data_at(&(t -> type), termtypeID(trm)) *
+            data_at(&(t -> content.Var), y) *
+            store_string(y, var)
+      */
       if (!strcmp(t->content.Var, src)) {
+        /*@ exists y var,
+            trm == TermVar(var) &&
+            data_at(&(t -> type), termtypeID(trm)) *
+            data_at(&(t -> content.Var), y) *
+            store_string(y, var)
+            which implies
+            store_term(t, trm)
+        */
         free_term(t);
         t = copy_term(den);
       }
@@ -62,11 +142,32 @@ term *subst_term(term *den, char *src, term *t)
       break;
     }
     case Apply: {
+      /*@ data_at(&(t -> type), termtypeID(trm)) *
+          store_term'(t, trm)
+          which implies
+          exists y z lt rt,
+            trm == TermApply(lt, rt) &&
+            data_at(&(t -> type), termtypeID(trm)) *
+            data_at(&(t -> content.Apply.left), y) *
+            data_at(&(t -> content.Apply.right), z) *
+            store_term(y, lt) * store_term(z, rt)
+      */
       t->content.Apply.left = subst_term(den, src, t->content.Apply.left);
       t->content.Apply.right = subst_term(den, src, t->content.Apply.right);
       break;
     }
     case Quant: {
+      /*@ data_at(&(t -> type), termtypeID(trm)) *
+          store_term'(t, trm)
+          which implies
+          exists y z qt qvar qterm,
+            trm == TermQuant(qt, qvar, qterm) &&
+            data_at(&(t -> type), termtypeID(trm)) *
+            data_at(&(t -> content.Quant.type), qtID(qt)) *
+            data_at(&(t -> content.Quant.var), y) *
+            data_at(&(t -> content.Quant.body), z) *
+            store_string(y, qvar) * store_term(z, qterm)
+      */
       if (strcmp(t->content.Quant.var, src)) {
         t->content.Quant.body = subst_term(den, src, t->content.Quant.body);
       }
