qcp/ast/VC/subst_goal_check.v
@@ -1,0 +1,6 @@
+Require Import subst_goal subst_proof_auto subst_proof_manual.
+
+Module VC_Correctness : VC_Correct.
+  Include subst_proof_auto.
+  Include subst_proof_manual.
+End VC_Correctness.
