qcp/ast/VC/subst_proof_auto.v
@@ -1,0 +1,119 @@
+Require Import Coq.ZArith.ZArith.
+Require Import Coq.Bool.Bool.
+Require Import Coq.Strings.String.
+Require Import Coq.Lists.List.
+Require Import Coq.Classes.RelationClasses.
+Require Import Coq.Classes.Morphisms.
+Require Import Coq.micromega.Psatz.
+Require Import Coq.Sorting.Permutation.
+From AUXLib Require Import int_auto Axioms Feq Idents List_lemma VMap.
+Require Import SetsClass.SetsClass. Import SetsNotation.
+From SimpleC.SL Require Import Mem SeparationLogic.
+Require Import subst_goal.
+Require Import Logic.LogicGenerator.demo932.Interface.
+Local Open Scope Z_scope.
+Local Open Scope sets.
+Local Open Scope string.
+Local Open Scope list.
+Require Import ast_lib.
+From SimpleC.EE Require Import ast_lib.
+From SimpleC.EE Require Import malloc.
+From SimpleC.EE Require Import sll_tmpl.
+Local Open Scope sac.
+
+Lemma proof_of_subst_var_safety_wit_1 : subst_var_safety_wit_1.
+Proof. Admitted. 
+
+Lemma proof_of_subst_var_safety_wit_2 : subst_var_safety_wit_2.
+Proof. Admitted. 
+
+Lemma proof_of_subst_var_safety_wit_3 : subst_var_safety_wit_3.
+Proof. Admitted. 
+
+Lemma proof_of_subst_var_safety_wit_4 : subst_var_safety_wit_4.
+Proof. Admitted. 
+
+Lemma proof_of_subst_var_partial_solve_wit_1 : subst_var_partial_solve_wit_1.
+Proof. Admitted. 
+
+Lemma proof_of_subst_var_partial_solve_wit_2 : subst_var_partial_solve_wit_2.
+Proof. Admitted. 
+
+Lemma proof_of_subst_var_partial_solve_wit_3 : subst_var_partial_solve_wit_3.
+Proof. Admitted. 
+
+Lemma proof_of_subst_var_partial_solve_wit_4 : subst_var_partial_solve_wit_4.
+Proof. Admitted. 
+
+Lemma proof_of_subst_var_partial_solve_wit_5 : subst_var_partial_solve_wit_5.
+Proof. Admitted. 
+
+Lemma proof_of_subst_var_partial_solve_wit_6 : subst_var_partial_solve_wit_6.
+Proof. Admitted. 
+
+Lemma proof_of_subst_var_partial_solve_wit_7 : subst_var_partial_solve_wit_7.
+Proof. Admitted. 
+
+Lemma proof_of_subst_var_partial_solve_wit_8 : subst_var_partial_solve_wit_8.
+Proof. Admitted. 
+
+Lemma proof_of_subst_var_partial_solve_wit_9 : subst_var_partial_solve_wit_9.
+Proof. Admitted. 
+
+Lemma proof_of_subst_var_partial_solve_wit_10 : subst_var_partial_solve_wit_10.
+Proof. Admitted. 
+
+Lemma proof_of_subst_var_partial_solve_wit_11 : subst_var_partial_solve_wit_11.
+Proof. Admitted. 
+
+Lemma proof_of_subst_term_safety_wit_1 : subst_term_safety_wit_1.
+Proof. Admitted. 
+
+Lemma proof_of_subst_term_safety_wit_2 : subst_term_safety_wit_2.
+Proof. Admitted. 
+
+Lemma proof_of_subst_term_safety_wit_3 : subst_term_safety_wit_3.
+Proof. Admitted. 
+
+Lemma proof_of_subst_term_safety_wit_4 : subst_term_safety_wit_4.
+Proof. Admitted. 
+
+Lemma proof_of_subst_term_partial_solve_wit_1 : subst_term_partial_solve_wit_1.
+Proof. Admitted. 
+
+Lemma proof_of_subst_term_partial_solve_wit_2 : subst_term_partial_solve_wit_2.
+Proof. Admitted. 
+
+Lemma proof_of_subst_term_partial_solve_wit_3 : subst_term_partial_solve_wit_3.
+Proof. Admitted. 
+
+Lemma proof_of_subst_term_partial_solve_wit_4_pure : subst_term_partial_solve_wit_4_pure.
+Proof. Admitted. 
+
+Lemma proof_of_subst_term_partial_solve_wit_4 : subst_term_partial_solve_wit_4.
+Proof. Admitted. 
+
+Lemma proof_of_subst_term_partial_solve_wit_5 : subst_term_partial_solve_wit_5.
+Proof. Admitted. 
+
+Lemma proof_of_subst_term_partial_solve_wit_6 : subst_term_partial_solve_wit_6.
+Proof. Admitted. 
+
+Lemma proof_of_subst_term_partial_solve_wit_7 : subst_term_partial_solve_wit_7.
+Proof. Admitted. 
+
+Lemma proof_of_subst_term_partial_solve_wit_8 : subst_term_partial_solve_wit_8.
+Proof. Admitted. 
+
+Lemma proof_of_subst_term_partial_solve_wit_9 : subst_term_partial_solve_wit_9.
+Proof. Admitted. 
+
+Lemma proof_of_subst_term_partial_solve_wit_10 : subst_term_partial_solve_wit_10.
+Proof. Admitted. 
+
+Lemma proof_of_subst_term_partial_solve_wit_11 : subst_term_partial_solve_wit_11.
+Proof. Admitted. 
+
+Lemma proof_of_subst_term_partial_solve_wit_12 : subst_term_partial_solve_wit_12.
+Proof. Admitted. 
+
