qcp/ast/VC/subst_proof_manual.v
@@ -1,0 +1,114 @@
+Require Import Coq.ZArith.ZArith.
+Require Import Coq.Bool.Bool.
+Require Import Coq.Strings.String.
+Require Import Coq.Lists.List.
+Require Import Coq.Classes.RelationClasses.
+Require Import Coq.Classes.Morphisms.
+Require Import Coq.micromega.Psatz.
+Require Import Coq.Sorting.Permutation.
+From AUXLib Require Import int_auto Axioms Feq Idents List_lemma VMap.
+Require Import SetsClass.SetsClass. Import SetsNotation.
+From SimpleC.SL Require Import Mem SeparationLogic.
+Require Import subst_goal.
+Require Import Logic.LogicGenerator.demo932.Interface.
+Local Open Scope Z_scope.
+Local Open Scope sets.
+Local Open Scope string.
+Local Open Scope list.
+Require Import ast_lib.
+Require Import Coq.Strings.String.
+Require Import ast_lib.
+From SimpleC.EE Require Import malloc.
+From SimpleC.EE Require Import sll_tmpl.
+Local Open Scope sac.
+
+Lemma proof_of_subst_var_return_wit_1_1 : subst_var_return_wit_1_1.
+Proof. Admitted. 
+
+Lemma proof_of_subst_var_return_wit_1_2 : subst_var_return_wit_1_2.
+Proof. Admitted. 
+
+Lemma proof_of_subst_var_return_wit_1_3 : subst_var_return_wit_1_3.
+Proof. Admitted. 
+
+Lemma proof_of_subst_var_return_wit_1_4 : subst_var_return_wit_1_4.
+Proof. Admitted. 
+
+Lemma proof_of_subst_var_return_wit_1_5 : subst_var_return_wit_1_5.
+Proof. Admitted. 
+
+Lemma proof_of_subst_var_return_wit_1_6 : subst_var_return_wit_1_6.
+Proof. Admitted. 
+
+Lemma proof_of_subst_var_return_wit_1_7 : subst_var_return_wit_1_7.
+Proof. Admitted. 
+
+Lemma proof_of_subst_var_partial_solve_wit_4_pure : subst_var_partial_solve_wit_4_pure.
+Proof. Admitted. 
+
+Lemma proof_of_subst_var_partial_solve_wit_7_pure : subst_var_partial_solve_wit_7_pure.
+Proof. Admitted. 
+
+Lemma proof_of_subst_var_partial_solve_wit_8_pure : subst_var_partial_solve_wit_8_pure.
+Proof. Admitted. 
+
+Lemma proof_of_subst_var_partial_solve_wit_11_pure : subst_var_partial_solve_wit_11_pure.
+Proof. Admitted. 
+
+Lemma proof_of_subst_var_which_implies_wit_1 : subst_var_which_implies_wit_1.
+Proof. Admitted. 
+
+Lemma proof_of_subst_var_which_implies_wit_2 : subst_var_which_implies_wit_2.
+Proof. Admitted. 
+
+Lemma proof_of_subst_var_which_implies_wit_3 : subst_var_which_implies_wit_3.
+Proof. Admitted. 
+
+Lemma proof_of_subst_var_which_implies_wit_4 : subst_var_which_implies_wit_4.
+Proof. Admitted. 
+
+Lemma proof_of_subst_term_return_wit_1_1 : subst_term_return_wit_1_1.
+Proof. Admitted. 
+
+Lemma proof_of_subst_term_return_wit_1_2 : subst_term_return_wit_1_2.
+Proof. Admitted. 
+
+Lemma proof_of_subst_term_return_wit_1_3 : subst_term_return_wit_1_3.
+Proof. Admitted. 
+
+Lemma proof_of_subst_term_return_wit_1_4 : subst_term_return_wit_1_4.
+Proof. Admitted. 
+
+Lemma proof_of_subst_term_return_wit_1_5 : subst_term_return_wit_1_5.
+Proof. Admitted. 
+
+Lemma proof_of_subst_term_return_wit_1_6 : subst_term_return_wit_1_6.
+Proof. Admitted. 
+
+Lemma proof_of_subst_term_return_wit_1_7 : subst_term_return_wit_1_7.
+Proof. Admitted. 
+
+Lemma proof_of_subst_term_partial_solve_wit_8_pure : subst_term_partial_solve_wit_8_pure.
+Proof. Admitted. 
+
+Lemma proof_of_subst_term_partial_solve_wit_9_pure : subst_term_partial_solve_wit_9_pure.
+Proof. Admitted. 
+
+Lemma proof_of_subst_term_partial_solve_wit_12_pure : subst_term_partial_solve_wit_12_pure.
+Proof. Admitted. 
+
+Lemma proof_of_subst_term_which_implies_wit_1 : subst_term_which_implies_wit_1.
+Proof. Admitted. 
+
+Lemma proof_of_subst_term_which_implies_wit_2 : subst_term_which_implies_wit_2.
+Proof. Admitted. 
+
+Lemma proof_of_subst_term_which_implies_wit_3 : subst_term_which_implies_wit_3.
+Proof. Admitted. 
+
+Lemma proof_of_subst_term_which_implies_wit_4 : subst_term_which_implies_wit_4.
+Proof. Admitted. 
+
+Lemma proof_of_subst_term_which_implies_wit_5 : subst_term_which_implies_wit_5.
+Proof. Admitted. 
+
